acl2/eval/eval-receive.lisp
@@ -7,7 +7,14 @@
 (define eval-receive ((s erl-state-p) (cls erl-clause-list-p))
   (declare (ignorable cls))
   :returns (mv (rs erl-state-p) (body expr-list-p))
-  (mv (update-erl-state->in s (make-erl-val-blocked)) nil)
+  (b* (((erl-state s) (erl-state-fix s))
+        (cls (erl-clause-list-fix cls))
+        ((mv (erl-state rs) body)      
+         (eval-clauses (list s.in) cls s))
+        ((if (equal (erl-val-kind rs.in) :reject)) (mv rs nil))
+        ((if (null body))
+         (mv (update-erl-state->in s (make-erl-val-blocked)) nil)))
+      (mv rs body))
   
   ///
     (defcong erl-state-equiv equal (eval-receive s cls) 1)
