acl2/scheduler/abstract.lisp
@@ -1,0 +1,178 @@
+(in-package "ACL2")
+(include-book "proc")
+(include-book "std/omaps/extensionality" :dir :system)
+
+(set-induction-depth-limit 1)
+
+; Possible Scheduling Steps ---------------------------------------------------
+
+(fty::deftagsum scheduling
+  (:deliver ((p1 pid-p) (p2 pid-p)))
+  (:run ((p pid-p)))
+  (:stutter ()))
+
+
+; Weakly Fair Abstract Scheduler ----------------------------------------------
+
+(encapsulate
+
+  (((schedule * ) => *))
+
+  ; Witness function
+
+  (local (define schedule ((net network-p))
+    :returns (s scheduling-p)
+    :verify-guards nil
+    :measure (acl2-count (network-fix net))
+    (b* ((net (network-fix net))
+         ((if (omap::emptyp net)) (make-scheduling-stutter))
+         (pid (omap::head-key net))
+         ((if (runnable? net pid)) (make-scheduling-run :p pid))
+         (outbox (proc->outbox (omap::lookup pid net)))
+         ((unless (omap::emptyp outbox)) (make-scheduling-deliver :p1 pid :p2 (omap::head-key outbox))))
+        (schedule (omap::tail net)))
+    :hints (("Goal" :in-theory (enable network-fix)))
+    ///
+      (defcong network-equiv equal (schedule net) 1)
+      (verify-guards schedule
+        :hints (("Goal" :in-theory (enable network-p))))))
+  
+  ; Theorems
+
+  (local (defrule crock-1
+    (implies (and (omap::assoc x m) (not (omap::assoc x (omap::tail m))))
+             (equal (omap::head-key m) x))))
+  
+  (defrule crock-2
+    (implies (network-p m) (network-p (omap::tail m)))
+    :enable network-p)
+  
+  (defrule crock-3
+    (implies (and (network-p m) (pid-p x) (omap::assoc x (omap::tail m)))
+             (equal (omap::lookup x m)
+                    (omap::lookup x (omap::tail m))))
+    :enable (network-p network-gen-p)
+
+    :use (:instance omap::lookup-of-tail-when-assoc-tail
+            (key x) (map m)))
+
+  (defrule scheduler-weakly-fair-when-runnable
+    (implies 
+      (and (pid-p pid)
+           (network-p net)
+           (omap::assoc pid net)
+           (runnable? net pid))
+      (not (equal (schedule net) (make-scheduling-stutter))))
+    :enable (schedule runnable? proc-runnable?)
+    :hints (("Subgoal *1/5" :use (:instance crock-1 (x pid) (m net)))))
+  
+  (defrule scheduler-weakly-fair-when-has-message
+    (implies 
+      (and (pid-p pid) (pid-p dst)
+           (network-p net)
+           (omap::assoc pid net)
+           (has-message-for-dst? net pid dst))
+      (not (equal (schedule net) (make-scheduling-stutter))))
+    :enable (schedule has-message-for-dst? proc-has-message-for-dst? proc->outbox)
+    :hints (("Subgoal *1/5" :use (:instance crock-1 (x pid) (m net)))
+            ("Subgoal *1/6" :use ((:instance crock-1 (x pid) (m net))))))
+  
+  
+  ; Theorems
+  (defrule return-type-of-schedule-step
+    (scheduler-step-p (schedule-step p)))
+  (defrule return-type-of-schedule-proc
+    (implies (and (network-p net) (not (terminated? net))) 
+             (pid-p (schedule-proc net)))
+    :enable (terminated? runnable?))
+  (defrule return-type-of-schedule-src
+    (implies (and (network-p net) (network-has-message? net))
+             (pid-p (schedule-src net)))
+    :enable (has-message? network-has-message?))
+  (defrule return-type-of-schedule-dst
+    (implies (and (proc-p src) (has-message? src))
+             (pid-p (schedule-dst src)))
+    :enable has-message?)
+  
+  ; schedule-proc
+  (defrule scheduled-pid-is-in-the-network
+    (implies
+      (and (network-p net) (not (terminated? net))) 
+      (omap::assoc (schedule-proc net) net))
+    :enable (terminated? runnable?))
+  
+  (local (defrule scheduled-pid-is-a-runnable-proc-tail
+    (implies
+      (and (network-p net) (not (terminated? net)) 
+           (omap::assoc (schedule-proc net) (omap::tail net))) 
+      (runnable? (omap::lookup (schedule-proc net) net)))
+    :enable (terminated? runnable? omap::lookup)
+    :induct (terminated? net)))
+  
+  (local (defrule scheduled-pid-is-in-the-network-head
+    (implies
+      (and (network-p net) (not (terminated? net)) 
+           (not (omap::assoc (schedule-proc net) (omap::tail net)))) 
+      (equal (omap::head-key net) (schedule-proc net)))
+    :enable (terminated? runnable? omap::lookup)
+    :induct (terminated? net)))
+  
+  (local (defrule scheduled-pid-is-a-runnable-proc-head
+    (implies
+      (and (network-p net) (not (terminated? net)) 
+           (not (omap::assoc (schedule-proc net) (omap::tail net)))) 
+      (runnable? (omap::lookup (schedule-proc net) net)))
+    :enable (terminated? runnable? omap::lookup)
+    :induct (terminated? net)))
+  
+  (defrule scheduled-pid-is-a-runnable-proc
+    (implies
+      (and (network-p net) (not (terminated? net))) 
+      (runnable? (omap::lookup (schedule-proc net) net)))
+    :cases ((omap::assoc (schedule-proc net) (omap::tail net)))
+    :disable schedule-proc)
+  
+  ; schedule-src
+  (defrule scheduled-src-is-in-the-network
+    (implies
+      (and (network-p net) (network-has-message? net)) 
+      (omap::assoc (schedule-src net) net))
+    :enable (network-has-message? has-message?))
+  
+  (local (defrule scheduled-src-has-a-message-tail
+    (implies
+      (and (network-p net) (network-has-message? net) 
+           (omap::assoc (schedule-src net) (omap::tail net))) 
+      (has-message? (omap::lookup (schedule-src net) net)))
+    :enable (network-has-message? has-message? omap::lookup)
+    :induct (network-has-message? net)))
+  
+  (local (defrule scheduled-src-is-in-the-network-head
+    (implies
+      (and (network-p net) (network-has-message? net)
+           (not (omap::assoc (schedule-src net) (omap::tail net)))) 
+      (equal (omap::head-key net) (schedule-src net)))
+    :enable (network-has-message? has-message? omap::lookup)
+    :induct (network-has-message? net)))
+  
+  (local (defrule scheduled-src-has-a-message-head
+    (implies
+      (and (network-p net) (network-has-message? net)
+           (not (omap::assoc (schedule-src net) (omap::tail net)))) 
+      (has-message? (omap::lookup (schedule-src net) net)))
+    :enable (network-has-message? has-message? omap::lookup)
+    :induct (network-has-message? net)))
+  
+  (defrule scheduled-src-has-a-message
+    (implies
+      (and (network-p net) (network-has-message? net))
+      (has-message? (omap::lookup (schedule-src net) net)))
+    :cases ((omap::assoc (schedule-src net) (omap::tail net)))
+    :disable schedule-src)
+  
+  ; schedule-dst
+  (defrule src-has-message-for-scheduled-dst
+    (implies
+      (and (proc-p p) (has-message? p)) 
+      (omap::assoc (schedule-dst p) (erl-state->outbox (proc->es p))))
+    :enable has-message?))
