acl2/scheduler/proc.lisp
@@ -1,0 +1,95 @@
+(in-package "ACL2")
+(include-book "../eval/top")
+
+; Erlang Process --------------------------------------------------------------
+
+(std::defenum proc-state-p
+  (:idle :terminated :receive-enter :receive-wait))
+
+(fty::defprod proc
+  (; state of the Erlang process
+   (ps proc-state-p :default :idle)
+
+   ; state of the Erlang program run by the process
+   (s erl-state-p :default (make-erl-state))
+
+   ; the messages received, but not yet tried on the next
+   ; receive. (this is only used to prevent receive loops)
+   (inbox-new erl-vlst-p :default nil)
+
+   ; messages that have been received and have already been
+   ; tried by the next receive.
+   (inbox-tried erl-vlst-p :default nil)
+   
+   ; the remaining computation
+   (klst erl-klst-p :default nil)))
+
+(define proc->pid ((p proc-p))
+  :returns (pid pid-p)
+  (b* ((p (proc-fix p)))
+      (erl-state->self (proc->s p)))
+  ///
+    (defcong proc-equiv equal (proc->pid p) 1))
+
+(define proc->outbox ((p proc-p))
+  :returns (o outbox-p)
+  (b* ((p (proc-fix p)))
+      (erl-state->outbox (proc->s p)))
+  ///
+    (defcong proc-equiv equal (proc->outbox p) 1))
+
+(define proc-runnable? ((p proc-p))
+  :returns (b booleanp)
+  (b* ((p (proc-fix p)))
+      (or (equal (proc->ps p) :idle)
+          (equal (proc->ps p) :receive)))
+  ///
+    (defcong proc-equiv equal (proc-runnable? p) 1))
+
+(define proc-has-message-for-dst? ((p proc-p) (dst pid-p))
+  (b* ((p (proc-fix p))
+       (dst (pid-fix dst)))
+      (and (erl-state->outbox (proc->s p))
+           (omap::assoc dst (erl-state->outbox (proc->s p)))))
+  ///
+    (defcong proc-equiv equal (proc-has-message-for-dst? p dst) 1)
+    (defcong pid-equiv equal (proc-has-message-for-dst? p dst) 2))
+
+(fty::defomap network-gen
+    :key-type pid-p
+    :val-type proc-p)
+
+(define wf-network-p ((n network-gen-p))
+  :enabled t
+  :returns (b booleanp)
+  :measure (acl2-count (network-gen-fix n))
+  (b* ((n (network-gen-fix n))
+       ((if (omap::emptyp n)) t))
+      (and (equal (omap::head-key n) (erl-state->self (proc->s (omap::head-val n))))
+           (wf-network-p (omap::tail n)))))
+
+(fty::defsubtype network
+  :supertype network-gen
+  :restriction (lambda (x) (wf-network-p x))
+  :fix-value nil)
+
+(define runnable? ((n network-p) (p pid-p))
+  :returns (b booleanp)
+  (b* ((n (network-fix n))
+       (p (pid-fix p)))
+      (and (omap::assoc p n)
+           (proc-runnable? (omap::lookup p n))))
+  ///
+    (defcong network-equiv equal (runnable? n p) 1)
+    (defcong proc-equiv equal (runnable? n p) 2))
+
+(define has-message-for-dst? ((net network-p) (src pid-p) (dst pid-p))
+  (b* ((net (network-fix net))
+       (src (pid-fix src))
+       (dst (pid-fix dst)))
+      (and (omap::assoc src net)
+           (proc-has-message-for-dst? (omap::lookup src net) dst)))
+  ///
+    (defcong network-equiv equal (has-message-for-dst? net src dst) 1)
+    (defcong pid-equiv equal (has-message-for-dst? net src dst) 2)
+    (defcong pid-equiv equal (has-message-for-dst? net src dst) 3))
